# Preamble
\usepackage{xcolor}
\definecolor{fore}{HTML}{544536}


# Equations

### HRS block

$$
\hat S_{X,b}(t,f) 
    = \frac{B}{K}\left| \sum_{n=0}^{B-1}
    \left[\sum_{k=0}^{K-1}\nu_{k}(t-b)\nu_{k}(n)\right] 
    x_b(n+b)e^{-i2\pi fn} \right|^2
$$

#### Sliding window

$$
\begin{aligned}
    \hat S_{X,B}^{sw}(t,f) &= \hat S_{X,b}\big(t(b),f\big) 
    \\&\\
    t(b) &= b + \lceil (B/2)\rceil 
    \\
    b &= t - \lceil (B/2)\rceil
\end{aligned}
$$

$$
\begin{aligned}
  t \in T(B) &\stackrel{\text{def}}{=} \Big\{t_0 , \dots, t_{B-1}\Big\}
\end{aligned}
$$

$$
\begin{aligned}
  t \in T(B) &\stackrel{\text{def}}{=} \Big\{t_0 , \dots, t_\beta\Big\}
\end{aligned}
$$

## MOdified Sgram

#### NSQI

$$
S_X(t + \tau,f) = \sum_{j=0}^{J-1} u_j(t,f)U_j(\tau)
$$

#### EigenProblem

$$
\alpha_j U_j(t) = N\sum_{\tau=0}^{N-1}
    \left|
        \frac{\sin\Big(N\pi(t-\tau)\Big)}{\sin\Big(\pi(t-\tau)\Big)}
    \right|^2 U_j(\tau)
$$
#### Approx NSQI vs Taylor Series

$$
\begin{aligned}
S_{b}(t,f) 
    &\approx \sum_{j=0}^{J_b} u_{j,b}(f)U_l(j-b)
\\&\\
    S_{b}(t,f)
    &\approx S_{b}\big(t(b),f\big) + S_{b}^{(1)}\big(t(b),f\big)\big(t-t(b)\big)
\end{aligned}
$$

#### NSQI == Taylor Series

$$
\sum_{j=0}^{J_b} u_{j,b}(f)U_l(j-b)
\approx 
S_{b}(t(b),f) + S_{b}^{(1)}(t(b),f)(t-t(b))
$$

#### ModSpec

$$
\hat S_{b}^{ms}(t(b),f) 
    = \frac{\frac{K}{\alpha_0}\sum_{t=b}^{b+B-1}\hat S_{b}(t,f)U_0(t-b)}
                    {\sum_{t=b}^{b+B-1} U_0(t-b)}.
$$
#### TD-Modspec

$$
\hat S^{ms (1)}_{b}(t(b),f) = 
    \frac{\frac{K}{\alpha_1}\sum_{t=b}^{b+B-1}\hat S_{b}(t,f)U_1(t-b)}
    {\sum_{t=b}^{b+B-1} U_1(t-b)(t-t(b))}
$$

## Boundary Correction

#### 1-BC

$$
\hat S_B^{\{1\}}(t,f) = 
    \begin{cases}
        \hat S^{ms}_{\beta}(t(\beta),f) + |t-t(\beta)|\hat S^{ms(1)}_{\beta}(t(\beta),f)  &\quad t > t_\beta \\&\\
        \hat S^{ms}_{b}(t(b),f) ;\quad  b = t-\lceil(B/2)\rceil                           &\quad t \in T(B) \\&\\
        \hat S^{ms}_{0}(t(0),f) - |t-t(0)|\hat S^{ms(1)}_{0}(t(0),f)                      &\quad t < t_0
    \end{cases} 
$$

#### 2-BC

$$
\hat S_B^{\{2\}}(t,f) = 
    \begin{cases}
        \hat S^{(0)}_{\beta}(t(\beta),f) 
            + |t-t(\beta)|\hat S^{(1)}_{\beta}(t(\beta),f)
            + \frac{|t-t(\beta)|^2}{2}\hat S^{(2)}_{\beta}(t(\beta),f)
            &\quad  t > t_\beta 
    \\&\\
        \hat S^{(0)}_{b}(t(b),f) ;\quad  b = t-\lceil(B/2)\rceil
            &\quad  t \in T(B)
    \\&\\
        \hat S^{(0)}_{0}(t(0),f) 
            - |t-t(0)|\hat S^{(1)}_{0}(t(0),f)
            - \frac{|t-t(0)|^2}{2}\hat S^{(2)}_{0}(t(0),f)
            &\quad  t < t_0,
    \end{cases}
$$

## UMP dissection

### GEST

$$
\begin{aligned}
  X(t) &= c(t)Y(t) 
  \\&\\
  S_X(t,f) &= c^{2}(t)Y(t)
\end{aligned}
$$

$$
S_X(t,f)= c^2(t)S_Y(f)
$$


$$
S_X(t,f)= g(t)S_Y(f)
$$

#### Rowsums: c2(t)

$$
\sum_{i=1}^{N_f} S_X(t,f_i)
           = g(t)\sum_{i=1}^{N_f} S_Y(f_i)
$$

#### setup gest

$$
\frac
  {\sum_{i=1}^{N_f} S_X(t_1,f_i)}
  {\sum_{i=1}^{N_f} S_X(t_2,f_i)}
= \frac
  {g(t_1)\sum_{i=1}^{N_f} S_Y(f_i)}
  {g(t_2)\sum_{i=1}^{N_f} S_Y(f_i)}
$$

$$
A_{t_1,t_2}
$$

$$
\sum_{j=1}^N g(t_i) = \sum_{j=1}^N A_{t_it_j}\,g(t_j)
$$

$$
\vec g = \frac{1}{N}A \vec g
$$


### YEST


$$
\sum_{t=1}^{N} S_X(t,f) = S_Y(f)\sum_{t=1}^{N}g(t)
$$

$$
\frac
  {\sum_{t=1}^{N} S_X(t,f_1)}
  {\sum_{t=1}^{N} S_X(t,f_2)}
= \frac
  {S_Y(f_1)\sum_{t=1}^{N}g(t)}
  {S_Y(f_2)\sum_{t=1}^{N}g(t)}
$$

$$
A_{f_1,f_2}
$$

$$
\vec S_Y = \frac{1}{N_f}A \vec S_Y
$$

$$
\hat g_1        \\
\hat S_{Y,1}    \\
\hat g_2        \\
\hat S_{Y,2}    \\
$$


## Smoothing

$$
\tilde S_X(t,f) = \hat g_2(t) \hat S_{Y,2}(f)
$$







